src/3d/Options.fsti
@@ -81,3 +81,5 @@ val get_save_z3_transcript: unit -> ML (option string)
 val get_test_checker: unit -> ML (option string)
 
 val get_z3_branch_depth: unit -> ML nat
+
+val get_skip_checks_in_z3_test_executable : unit -> ML bool
